started defining a reflected type for specs

theories/Spec.v
@@ -1,12 +1,14 @@
 
-(*** Specs represented as dependent records ***)
+(*** Modeling specs and morphisms as Coq terms ***)
 
 Require Import List.
 Import ListNotations.
 Require Import String.
 
+(*
 Add LoadPath "." as Specware.
 Require Import Specware.Util.
+*)
 
 
 (* Define the type of fields in one place, so we can change it later *)
@@ -15,75 +17,237 @@ Definition Field : Set := string.
 Definition Field_dec : forall (f1 f2 : Field), {f1=f2} + {f1<>f2} := string_dec.
 
 
-(*** Signatures ***)
+(*** The inductive type of specs ***)
 
-(* A signature is essentially a structuring device for describing a
-   dependent record type. The type Sig S describes a signature whose
-   models are the elements of type S. *)
-Inductive Sig : Type -> Type :=
-| Sig_Empty : Sig unit
-| Sig_AddOp S (s: Sig S) (f : Field) (A : S -> Type) : Sig { s:S & A s }
-| Sig_AddAxiom S (s: Sig S) (f : Field) (P : S -> Prop) : Sig { s:S | P s }
-| Sig_Import S1 (s1: Sig S1) S2 (s2: Sig S2) : Sig (S1 * S2)
+Inductive Spec : Type :=
+(* The base case contains the names and types of the axioms *)
+| Spec_Axioms (axioms : list (Field * Prop))
+(* Declared op: the rest of the spec can refer to the op *)
+| Spec_DeclOp (f : Field) (T : Type) (rest : T -> Spec)
+(* Defined op: gives an element of the type *)
+| Spec_DefOp (f : Field) (T : Type) (t : T) (rest : Spec)
 .
 
-(* The op fields of a signature *)
-Fixpoint op_fields S (s: Sig S) : list Field :=
-  match s in Sig S with
-    | Sig_Empty => []
-    | Sig_AddOp S' s' f _ => f :: op_fields S' s'
-    | Sig_AddAxiom S' s' _ _ => op_fields S' s'
-    | Sig_Import S1 s1 S2 s2 => op_fields S1 s1 ++ op_fields S2 s2
+(*
+Inductive Spec : list string -> Type :=
+(* The base case contains the names and types of the axioms *)
+| Spec_Axioms (axioms : list (Field * Prop)) : Spec []
+(* Declared op: the rest of the spec can refer to the op *)
+| Spec_DeclOp flds f (T : Type) (rest : T -> Spec flds)
+  : Spec (f :: flds)
+(* Defined op: gives an element of the type *)
+| Spec_DefOp flds f (T : Type) (t : T) (rest : Spec flds)
+  : Spec (f :: flds)
+.
+*)
+
+(*** The models of a spec ***)
+
+Definition Any : Type := { T : Type & T }.
+Definition mkAny (T:Type) (t:T) : Any := existT (fun T => T) T t.
+Definition dummyAny : Any := mkAny _ tt.
+
+Definition Model := list (Field * Any).
+
+Fixpoint model_proj f model : option Any :=
+  match model with
+    | [] => None
+    | (f', any) :: model' =>
+      if Field_dec f f' then Some any else
+        model_proj f model'
   end.
 
-(* The data (non-proof) fields of a signature *)
-Fixpoint axiom_fields S (s: Sig S) : list Field :=
-  match s in Sig S with
-    | Sig_Empty => []
-    | Sig_AddOp S' s' _ _ => axiom_fields S' s'
-    | Sig_AddAxiom S' s' f _ => f :: axiom_fields S' s'
-    | Sig_Import S1 s1 S2 s2 => axiom_fields S1 s1 ++ axiom_fields S2 s2
+Fixpoint combine_axioms (axioms : list (Field * Prop)) : Prop :=
+  fold_left (fun P1 f_P2 => and P1 (snd f_P2)) axioms True.
+
+(* NOTE: this is in Type because we need to compute the model elements *)
+Fixpoint IsModel (model:Model) (s:Spec) : Prop :=
+  match s with
+    | Spec_Axioms axioms => combine_axioms axioms
+    | Spec_DeclOp f T rest =>
+      exists t, model_proj f model = Some (mkAny T t) /\ IsModel model (rest t)
+    | Spec_DefOp f T t rest =>
+      model_proj f model = Some (mkAny T t) /\ IsModel model rest
   end.
 
 
-(*** Model projections ***)
+(*** Field maps ***)
 
-Definition Any := { A : Type & A}.
-Definition mkAny A a : Any := existT id A a.
+Definition FMap := list (Field * Field).
 
-Program Fixpoint model_proj S (s:Sig S) : { f: Field | In f (op_fields S s) } -> S -> Any :=
-  match s in Sig S return { f: Field | In f (op_fields S s) } -> S -> Any with
-    | Sig_Empty =>
-      fun f _ => match proj2_sig f with end
-    | Sig_AddOp S' s' f' A =>
-      fun f M =>
-        match Field_dec f f' with
-          | left _ => mkAny _ (projT2 M)
-          | right neq =>
-            model_proj S' s' f (projT1 M)
-        end
-    | Sig_AddAxiom S' s' _ _ =>
-      fun f M => model_proj S' s' f (proj1_sig M)
-    | Sig_Import S1 s1 S2 s2 =>
-      fun f M =>
-        match in_dec Field_dec f (op_fields S1 s1) with
-          | left in1 => model_proj S1 s1 f (fst M)
-          | right not_in1 => model_proj S2 s2 f (snd M)
-        end
+(*
+Definition FMap := { l : list (Field * Field) | NoDup (map fst l) }.
+
+Lemma NoDup_tail A (x:A) l : NoDup (x::l) -> NoDup l.
+  intro nd. apply (NoDup_remove_1 [] l x). assumption.
+Qed.
+*)
+
+Fixpoint apply_fmap (m : FMap) (f : Field) : Field :=
+  match m with
+    | [] => f
+    | (f_in, f_out) :: m' =>
+      if Field_dec f f_in then f_out else apply_fmap m' f
   end.
-Obligation 1.
-destruct H; [ elimtype False; apply neq; symmetry | ]; assumption.
-Defined.
-Obligation 3.
-destruct (in_app_or _ _ _ H); [ elimtype False; apply not_in1 | ]; assumption.
-Defined.
+
+Definition fmap_id : FMap := [].
+
+Lemma fmap_id_ok f : apply_fmap fmap_id f = f.
+  reflexivity.
+Qed.
+
+Fixpoint fmap_compose (m2 m1 : FMap) : FMap :=
+  match m1 with
+    | [] => m2
+    | (f_in, f_out) :: m1' =>
+      (f_in, apply_fmap m2 f_out) :: fmap_compose m2 m1'
+  end.
+
+Lemma fmap_compose_ok m2 m1 f :
+  apply_fmap (fmap_compose m2 m1) f = apply_fmap m2 (apply_fmap m1 f).
+  induction m1.
+  reflexivity.
+  destruct a.
+  unfold apply_fmap; unfold fmap_compose; fold fmap_compose; fold apply_fmap.
+  destruct (Field_dec f f0).
+  reflexivity.
+  assumption.
+Qed.
+
+Definition fmap_dom (m : FMap) : list Field := map fst m.
+
+Lemma reverse_fmap m f1 f2 :
+  apply_fmap m f1 = f2 -> f1 = f2 \/ In f1 (fmap_dom m).
+  admit. (* FIXME HERE *)
+Qed.
 
 
 (*** Morphisms ***)
 
-Definition IsMorphism (g: Field -> Field) S1 (s1:Sig S1) S2 (s2:Sig S2) : Prop :=
-  exists embed (embed_fields :
-                  forall f, In f (op_fields S1 s1) ->
-                            In (g f) (op_fields S2 s2)),
-    forall f i M2, model_proj S1 s1 (exist _ f i) (embed M2) =
-                   model_proj S2 s2 (exist _ (g f) (embed_fields f i)) M2.
+Fixpoint unmap_model (m : FMap) (model:Model) : Model := FIXME HERE
+
+Fixpoint IsMappedModel (m : FMap) (model:Model) (s:Spec) : Prop :=
+  match s with
+    | Spec_Axioms axioms => combine_axioms axioms
+    | Spec_DeclOp f T rest =>
+      exists t,
+        model_proj (apply_fmap m f) model = Some (mkAny T t)
+        /\ IsMappedModel m model (rest t)
+    | Spec_DefOp f T t rest =>
+      model_proj (apply_fmap m f) model = Some (mkAny T t)
+      /\ IsMappedModel m model rest
+  end.
+
+Definition IsMorphism m (source target : Spec) : Prop :=
+  forall model, IsModel model target -> IsMappedModel m model source.
+
+
+Lemma IsMappedModel_id model s : IsModel model s <-> IsMappedModel fmap_id model s.
+  split; induction s;
+  unfold IsModel; fold IsModel; unfold IsMappedModel; fold IsMappedModel; intro.
+  assumption.
+  destruct H0; destruct H0; exists x; split; [ | apply H]; assumption.
+  destruct H; split; [ | apply IHs ]; assumption.
+  assumption.
+  destruct H0; destruct H0; exists x; split; [ | apply H]; assumption.
+  destruct H; split; [ | apply IHs ]; assumption.
+Qed.
+
+Theorem morphism_refl spec : IsMorphism fmap_id spec spec.
+  intros model ism; apply IsMappedModel_id; assumption.
+Qed.
+
+(* Need a model (or a mapped model) to extract the fields from a spec *)
+(* Argh, needs UIP! *)
+(*
+Definition spec_fields m model spec : IsMappedModel m model spec -> list Field.
+  induction spec; unfold IsMappedModel; fold IsMappedModel; intro ism.
+  exact [].
+  destruct (model_proj (m f) model).
+  destruct a. assert (x = T).
+  destruct ism; destruct H; injection H; intros; assumption.
+  revert p ism; rewrite H; intros.
+  assert (IsMappedModel m model (rest p)).
+  destruct ism; 
+*)
+(*
+Fixpoint spec_fields m model spec : IsMappedModel m model spec -> list Field :=
+  match spec with
+    | Spec_Axioms _ => fun _ => []
+    | Spec_DeclOp f T rest =>
+*)
+
+
+Definition unmap_model (m : Field -> Field) (model:Model) (s:Spec) :
+  IsMappedModel m model s -> {model' | IsModel model' s }.
+  induction s; unfold IsMappedModel; fold IsMappedModel;
+  unfold IsModel; fold IsModel; intro ism.
+  exists []; assumption.
+  case_eq (model_proj (m f) model); intros.
+  destruct a. assert (x = T).
+  destruct ism; destruct H0; rewrite H in H0;
+    injection H0; intros; assumption.
+  revert p H; rewrite H0; intros.
+  destruct (X p).
+  
+
+  exists (m f, a).
+
+
+Fixpoint unmap_model (m : Field -> Field) (model:Model) (s:Spec) :
+  IsMappedModel m model s -> Model :=
+  match s with
+    | Spec_Axioms axioms => fun _ => x[]
+    | Spec_DeclOp f T rest =>
+      fun ism =>
+
+
+(*** FIXME: Old stuff below... ***)
+
+Fixpoint spec_model (spec:Spec) : Type :=
+  match spec with
+    | Spec_Axioms axioms =>
+      combine_axioms axioms
+    | Spec_DeclOp _ T rest =>
+      { t : T & spec_model (rest t)}
+    | Spec_DefOp _ _ _ rest => spec_model rest
+  end.
+
+
+(*** Project an op from a model of a spec ***)
+
+Fixpoint model_proj f spec : spec_model spec -> { T : Type & T } :=
+  match spec  with
+    | Spec_Axioms _ => fun _ => existT (fun T => T) unit tt
+    | Spec_DeclOp f' T rest =>
+      fun model =>
+        if Field_dec f f' then (existT (fun T => T) T (projT1 model))
+      else model_proj f (rest (projT1 model)) (projT2 model)
+    | Spec_DefOp f' T t rest =>
+      fun model =>
+        if Field_dec f f' then existT _ T t
+        else model_proj f rest model
+  end.
+
+
+(*** Whether a field function defines a morphism ***)
+
+(* Note: the co-domain comes first in IsMorphism, because it does not vary *)
+(*
+Inductive IsMorphism (m : Field -> Field) (s_codom : Spec) : Spec -> Prop :=
+| IsMorphism_Axioms 
+*)
+
+Fixpoint IsMorphModel (m : Field -> Field)
+         (source target : Spec) (t_model : Model) : Prop :=
+  match source with
+    | Spec_Axioms axioms =>
+      combine_axioms axioms
+    | Spec_DeclOp f T rest =>
+      
+
+Fixpoint IsMorphism (m : Field -> Field) (source target : Spec) : Prop :=
+  match source with
+    | Spec_Axioms axioms =>
+      combine_axioms axioms
+    | Spec_DeclOp f T rest =>
